floyd/align_compatible_dec.v
@@ -1,0 +1,98 @@
+Require Import VST.floyd.base2.
+Require Import VST.floyd.client_lemmas.
+Require Import VST.floyd.fieldlist.
+Require Import VST.floyd.type_induction.
+Require Import VST.floyd.nested_pred_lemmas.
+Open Scope Z.
+
+Module Type ACR_DEC.
+
+  Parameter align_compatible_rec_dec:
+    forall {cs: compspecs},
+      forall t z, {align_compatible_rec cenv_cs t z} + {~ align_compatible_rec cenv_cs t z}.
+
+End ACR_DEC.
+
+Module align_compatible_rec_dec: ACR_DEC.
+
+Section align_compatible_rec_dec.
+
+Context {cs: compspecs}.
+
+Definition dec_type := sigT (fun P: Z -> Prop => forall z: Z, {P z} + {~ P z}).
+
+Definition dec_by_value (ch: memory_chunk): dec_type :=
+  existT (fun P: Z -> Prop => forall z: Z, {P z} + {~ P z}) (fun z => (Memdata.align_chunk ch | z)) (fun z => Zdivide_dec (Memdata.align_chunk ch) z (Memdata.align_chunk_pos _)).
+
+Definition dec_False: dec_type :=
+  existT (fun P: Z -> Prop => forall z: Z, {P z} + {~ P z}) (fun z => False) (fun z => right (fun H => H)).
+
+Definition dec_True: dec_type :=
+  existT (fun P: Z -> Prop => forall z: Z, {P z} + {~ P z}) (fun z => True) (fun z => left I).
+(*
+Definition dec_aux_struct_field (denv: PTree.t dec_type) (i: positive) (m: members): dec_type :=
+  match field_type i m, field_offset cenv_cs i m with
+  | Errors.OK t, Errors.OK ofs => existT (fun P: Z -> Prop => forall z: Z, {P z} + {~ P z}) (fun z => projT1 (dec_aux denv t) (z + ofs)) (fun z => projT2 (dec_aux denv t) (z + ofs))
+  | _, _ => dec_False
+  end.
+
+Definition dec_aux_union_field (denv: PTree.t dec_type) (i: positive) (m: members): dec_type :=
+  match field_type i m with
+  | Errors.OK t => dec_aux denv t
+  | _ => dec_False
+  end.
+
+Fixpoint dec_aux_struct_composite (denv: PTree.t dec_type) (m_rec m: members): dec_type :=
+  match m_rec with
+  | nil => dec_True
+  | (i, _) :: m_rec' => existT (fun P: Z -> Prop => forall z: Z, {P z} + {~ P z}) (fun z => projT1 (dec_aux_struct_field denv i m) z /\ projT1 (dec_aux_struct_composite denv m_rec' m) z) (fun z => sumbool_dec_and (projT2 (dec_aux_struct_field denv i m) z) (projT2 (dec_aux_struct_composite denv m_rec' m) z))
+  end.
+
+Fixpoint dec_aux_union_composite (denv: PTree.t dec_type) (m_rec m: members): dec_type :=
+  match m_rec with
+  | nil => dec_True
+  | (i, _) :: m_rec' => existT (fun P: Z -> Prop => forall z: Z, {P z} + {~ P z}) (fun z => projT1 (dec_aux_union_field denv i m) z /\ projT1 (dec_aux_union_composite denv m_rec' m) z) (fun z => sumbool_dec_and (projT2 (dec_aux_union_field denv i m) z) (projT2 (dec_aux_union_composite denv m_rec' m) z))
+  end.
+
+
+Definition dec_aux: type -> dec_type.
+  refine (type_func (fun _ => dec_type) _ _ _ _).
+  + intro t.
+    exact (match access_mode t with
+           | By_value ch => dec_by_value ch
+           | _ => dec_False
+           end).
+  + intros t' n _ d.
+    exact (existT (fun P: Z -> Prop => forall z: Z, {P z} + {~ P z}) (fun z => forall i, 0 <= i < n -> projT1 d (z + sizeof t' * i)) (fun z => Zrange_pred_dec (fun i => projT1 d (z + sizeof t' * i)) (fun i => projT2 d (z + sizeof t' * i)) 0 n)).
+  + intros id _ D.
+    unfold FT_aux in D.
+    
+
+
+Definition dec_aux_composite (denv: PTree.t dec_type) (su: struct_or_union) (m: members): dec_type :=
+  match su with
+  | Struct => dec_aux_struct_composite denv m m
+  | Union => dec_aux_union_composite denv m m
+  end.
+
+Definition dec_aux_env : PTree.t dec_type :=
+  let l := composite_reorder.rebuild_composite_elements cenv in
+  fold_right (fun (ic: positive * composite) (T0: PTree.t dec_type) => let (i, co) := ic in let T := T0 in PTree.set i (dec_aux_composite T (co_su co) (co_members co)) T) (PTree.empty _) l.
+
+ *)
+
+Lemma align_compatible_rec_dec: forall t z, {align_compatible_rec cenv_cs t z} + {~ align_compatible_rec cenv_cs t z}.
+Admitted.
+
+End align_compatible_rec_dec.
+
+End align_compatible_rec_dec.
+
+Lemma align_compatible_dec: forall {cs: compspecs} t p, {align_compatible t p} + {~ align_compatible t p}.
+Proof.
+  intros.
+  destruct p; try solve [left; unfold align_compatible; simpl; tauto].
+  simpl.
+  apply align_compatible_rec_dec.align_compatible_rec_dec.
+Qed.
+
